Work on MyLean/Omega.lean

MyLean/Omega.lean
@@ -111,156 +111,156 @@ theorem frequently_leads_to_frequently {p q : Set X}
 
 end Sequence
 
-section Automaton
+section Automata
 
-class Automaton (A : Type*) where
+class Automata (A : Type*) where
   State : Type*
   init : Set State
   next : State → A → Set State
 
 variable {A : Type*}
 
-def IsFinite (M : Automaton A) : Prop := Finite A ∧ Finite M.State
+def IsFinite (M : Automata A) : Prop := Finite A ∧ Finite M.State
 
-def Deterministic (M : Automaton A) : Prop :=
+def Deterministic (M : Automata A) : Prop :=
   M.init.ncard = 1 ∧ ∀ s a, (M.next s a).ncard = 1
 
-def FinRun (M : Automaton A) (n : ℕ) (as : Fin n → A) (ss : Fin (n + 1) → M.State) :=
+def FinRun (M : Automata A) (n : ℕ) (as : Fin n → A) (ss : Fin (n + 1) → M.State) :=
   ss 0 ∈ M.init ∧ ∀ k : Fin n, ss (k + 1) ∈ M.next (ss k) (as k)
 
-def InfRun (M : Automaton A) (as : ℕ → A) (ss : ℕ → M.State) :=
+def InfRun (M : Automata A) (as : ℕ → A) (ss : ℕ → M.State) :=
   ss 0 ∈ M.init ∧ ∀ k : ℕ, ss (k + 1) ∈ M.next (ss k) (as k)
 
-def FinAccept (M : Automaton A) (acc : Set M.State) (n : ℕ) (as : Fin n → A) :=
+def FinAccept (M : Automata A) (acc : Set M.State) (n : ℕ) (as : Fin n → A) :=
   ∃ ss : Fin (n + 1) → M.State, FinRun M n as ss ∧ ss n ∈ acc
 
-def BuchiAccept (M : Automaton A) (acc : Set M.State) (as : ℕ → A) :=
+def BuchiAccept (M : Automata A) (acc : Set M.State) (as : ℕ → A) :=
   ∃ ss : ℕ → M.State, InfRun M as ss ∧ ∃ᶠ k in atTop, ss k ∈ acc
 
-def MullerAccept (M : Automaton A) (accSet : Set (Set M.State)) (as : ℕ → A) :=
+def MullerAccept (M : Automata A) (accSet : Set (Set M.State)) (as : ℕ → A) :=
   ∃ ss : ℕ → M.State, InfRun M as ss ∧ ∃ acc ∈ accSet, ∀ s, s ∈ acc ↔ (∃ᶠ k in atTop, ss k = s)
 
-def RabinAccept (M : Automaton A) (accPairs : Set (Set M.State × Set M.State)) (as : ℕ → A) :=
+def RabinAccept (M : Automata A) (accPairs : Set (Set M.State × Set M.State)) (as : ℕ → A) :=
   ∃ ss : ℕ → M.State, InfRun M as ss ∧ ∃ pair ∈ accPairs, (∃ᶠ k in atTop, ss k ∈ pair.1) ∧ (∀ᶠ k in atTop, ss k ∉ pair.2)
 
-def StreettAccept (M : Automaton A) (accPairs : Set (Set M.State × Set M.State)) (as : ℕ → A) :=
+def StreettAccept (M : Automata A) (accPairs : Set (Set M.State × Set M.State)) (as : ℕ → A) :=
   ∃ ss : ℕ → M.State, InfRun M as ss ∧ ∀ pair ∈ accPairs, (∃ᶠ k in atTop, ss k ∈ pair.1) → (∃ᶠ k in atTop, ss k ∈ pair.2)
 
-def AcceptedLang (M : Automaton A) (acc : Set M.State) : Set (List A) :=
+def AcceptedLang (M : Automata A) (acc : Set M.State) : Set (List A) :=
   { al | ∃ n as, FinAccept M acc n as ∧ al = List.ofFn as }
 
-def AcceptedOmegaLang (M : Automaton A) (acc : Set M.State) : Set (ℕ → A) :=
+def AcceptedOmegaLang (M : Automata A) (acc : Set M.State) : Set (ℕ → A) :=
   { as | BuchiAccept M acc as }
 
-end Automaton
+end Automata
 
-section AutomatonSum
+section AutomataSum
 
 variable {I A : Type*}
 
-def AutomatonSum (M : I → Automaton A) : Automaton A where
+def AutomataSum (M : I → Automata A) : Automata A where
   State := Σ i : I, (M i).State
   init := ⋃ i : I, Sigma.mk i '' (M i).init
   next := fun ⟨i, s⟩ a ↦ Sigma.mk i '' (M i).next s a
 
-variable (M : I → Automaton A)
+variable (M : I → Automata A)
 
-theorem automaton_sum_fin_run (n : ℕ) (as : Fin n → A) (ss : Fin (n + 1) → (AutomatonSum M).State) :
-    FinRun (AutomatonSum M) n as ss ↔ ∃ i ss_i, FinRun (M i) n as ss_i ∧ ss = (Sigma.mk i) ∘ ss_i := by
+theorem Automata_sum_fin_run (n : ℕ) (as : Fin n → A) (ss : Fin (n + 1) → (AutomataSum M).State) :
+    FinRun (AutomataSum M) n as ss ↔ ∃ i ss_i, FinRun (M i) n as ss_i ∧ ss = (Sigma.mk i) ∘ ss_i := by
   constructor
   · rintro ⟨h_init, h_next⟩
     have := h_init
-    simp [AutomatonSum, Automaton.init] at this
+    simp [AutomataSum, Automata.init] at this
     rcases this with ⟨i, s0, h_s0_init, h_s0_ss⟩
     have h_ss_exists : ∀ k : Fin (n + 1), ∃ sk : (M i).State, ss k = Sigma.mk i sk := by
       intro k ; induction' k using Fin.induction with k h_k
       · use s0 ; rw [h_s0_ss]
       rcases h_k with ⟨sk, h_sk⟩
       have h_next_k := h_next k
-      simp [AutomatonSum, h_sk] at h_next_k
+      simp [AutomataSum, h_sk] at h_next_k
       rcases h_next_k with ⟨sk', h_sk'⟩
       use sk' ; simp [h_sk'.2]
     choose ss_i h_ss_i using h_ss_exists
     use i, ss_i
     constructor
     · constructor
-      · rw [h_ss_i 0, Automaton.init] at h_init
-        simp [AutomatonSum] at h_init
+      · rw [h_ss_i 0, Automata.init] at h_init
+        simp [AutomataSum] at h_init
         obtain ⟨i, s', h_s', rfl, h_eq⟩ := h_init
         rw [heq_eq_eq] at h_eq
         rwa [h_eq] at h_s'
       · intro k
         have h_next_k := h_next k
         rw [h_ss_i k, h_ss_i (k + 1)] at h_next_k
-        simp [AutomatonSum] at h_next_k
+        simp [AutomataSum] at h_next_k
         simpa
     · ext k ; rw [h_ss_i k] ; simp
   · rintro ⟨i, ss_i, h_run, h_ss⟩
-    simp [h_ss, AutomatonSum]
+    simp [h_ss, AutomataSum]
     constructor
-    · simp [Automaton.init]
+    · simp [Automata.init]
       use i, (ss_i 0)
       simp ; exact h_run.1
     · intro k
-      simp [Automaton.next]
+      simp [Automata.next]
       have h_k := h_run.2 k
       simp at h_k
       exact h_k
 
-theorem automaton_sum_inf_run (as : ℕ → A) (ss : ℕ → (AutomatonSum M).State) :
-    InfRun (AutomatonSum M) as ss ↔ ∃ i ss_i, InfRun (M i) as ss_i ∧ ss = (Sigma.mk i) ∘ ss_i := by
+theorem Automata_sum_inf_run (as : ℕ → A) (ss : ℕ → (AutomataSum M).State) :
+    InfRun (AutomataSum M) as ss ↔ ∃ i ss_i, InfRun (M i) as ss_i ∧ ss = (Sigma.mk i) ∘ ss_i := by
   constructor
   · rintro ⟨h_init, h_next⟩
     have := h_init
-    simp [AutomatonSum, Automaton.init] at this
+    simp [AutomataSum, Automata.init] at this
     rcases this with ⟨i, s0, h_s0_init, h_s0_ss⟩
     have h_ss_exists : ∀ k, ∃ sk : (M i).State, ss k = Sigma.mk i sk := by
       intro k ; induction' k with k h_k
       · use s0 ; rw [h_s0_ss]
       rcases h_k with ⟨sk, h_sk⟩
       have h_next_k := h_next k
-      simp [AutomatonSum, h_sk] at h_next_k
+      simp [AutomataSum, h_sk] at h_next_k
       rcases h_next_k with ⟨sk', h_sk'⟩
       use sk' ; simp [h_sk'.2]
     choose ss_i h_ss_i using h_ss_exists
     use i, ss_i
     constructor
     · constructor
-      · rw [h_ss_i 0, Automaton.init] at h_init
-        simp [AutomatonSum] at h_init
+      · rw [h_ss_i 0, Automata.init] at h_init
+        simp [AutomataSum] at h_init
         obtain ⟨i, s', h_s', rfl, h_eq⟩ := h_init
         rw [heq_eq_eq] at h_eq
         rwa [h_eq] at h_s'
       · intro k
         have h_next_k := h_next k
         rw [h_ss_i k, h_ss_i (k + 1)] at h_next_k
-        simp [AutomatonSum] at h_next_k
+        simp [AutomataSum] at h_next_k
         assumption
     · ext k ; rw [h_ss_i k] ; simp
   · rintro ⟨i, ss_i, h_run, h_ss⟩
-    simp [h_ss, AutomatonSum]
+    simp [h_ss, AutomataSum]
     constructor
-    · simp [Automaton.init]
+    · simp [Automata.init]
       use i, (ss_i 0)
       simp ; exact h_run.1
     · intro k
-      simp [Automaton.next]
+      simp [Automata.next]
       exact h_run.2 k
 
-end AutomatonSum
+end AutomataSum
 
 section AcceptedLangUnion
 
-variable {I A : Type*} (M : I → Automaton A) (acc : (i : I) → Set ((M i).State))
+variable {I A : Type*} (M : I → Automata A) (acc : (i : I) → Set ((M i).State))
 
-def AutomatonSum_Acc : Set (AutomatonSum M).State := ⋃ i : I, Sigma.mk i '' acc i
+def AutomataSum_Acc : Set (AutomataSum M).State := ⋃ i : I, Sigma.mk i '' acc i
 
 theorem accepted_lang_union :
-    AcceptedLang (AutomatonSum M) (AutomatonSum_Acc M acc) = ⋃ i : I, AcceptedLang (M i) (acc i) := by
-  ext al ; simp [AutomatonSum_Acc, AcceptedLang, FinAccept]
+    AcceptedLang (AutomataSum M) (AutomataSum_Acc M acc) = ⋃ i : I, AcceptedLang (M i) (acc i) := by
+  ext al ; simp [AutomataSum_Acc, AcceptedLang, FinAccept]
   constructor
   · rintro ⟨n, as, ⟨ss, h_run, h_acc⟩, h_al⟩
-    obtain ⟨i, ss_i, h_run_i, h_ss_i⟩ := (automaton_sum_fin_run M n as ss).mp h_run
+    obtain ⟨i, ss_i, h_run_i, h_ss_i⟩ := (Automata_sum_fin_run M n as ss).mp h_run
     use i, n, as
     constructor
     · use ss_i
@@ -278,18 +278,18 @@ theorem accepted_lang_union :
     constructor
     · use ((Sigma.mk i) ∘ ss_i)
       constructor
-      · apply (automaton_sum_fin_run M n as ((Sigma.mk i) ∘ ss_i)).mpr
+      · apply (Automata_sum_fin_run M n as ((Sigma.mk i) ∘ ss_i)).mpr
         use i, ss_i
       · use i, ss_i (Fin.last n)
         simpa
     · assumption
 
 theorem accepted_omega_lang_union :
-    AcceptedOmegaLang (AutomatonSum M) (AutomatonSum_Acc M acc) = ⋃ i : I, AcceptedOmegaLang (M i) (acc i) := by
-  ext as ; simp [AutomatonSum_Acc, AcceptedOmegaLang, BuchiAccept]
+    AcceptedOmegaLang (AutomataSum M) (AutomataSum_Acc M acc) = ⋃ i : I, AcceptedOmegaLang (M i) (acc i) := by
+  ext as ; simp [AutomataSum_Acc, AcceptedOmegaLang, BuchiAccept]
   constructor
   · rintro ⟨ss, h_run, h_inf⟩
-    obtain ⟨i, ss_i, h_run_i, h_ss_i⟩ := (automaton_sum_inf_run M as ss).mp h_run
+    obtain ⟨i, ss_i, h_run_i, h_ss_i⟩ := (Automata_sum_inf_run M as ss).mp h_run
     use i, ss_i
     constructor
     · assumption
@@ -307,10 +307,10 @@ theorem accepted_omega_lang_union :
   · rintro ⟨i, ss_i, h_run_i, h_inf_i⟩
     use ((Sigma.mk i) ∘ ss_i)
     constructor
-    · apply (automaton_sum_inf_run M as ((Sigma.mk i) ∘ ss_i)).mpr
+    · apply (Automata_sum_inf_run M as ((Sigma.mk i) ∘ ss_i)).mpr
       use i, ss_i
     · let p k := ss_i k ∈ acc i
-      let q k := ∃ i', ∃ si' ∈ acc i', ⟨i', si'⟩ = ((Sigma.mk i ∘ ss_i) k : (AutomatonSum M).State)
+      let q k := ∃ i', ∃ si' ∈ acc i', ⟨i', si'⟩ = ((Sigma.mk i ∘ ss_i) k : (AutomataSum M).State)
       have h_p : ∃ᶠ k in atTop, p k := by assumption
       have h_pq : ∀ k, p k → q k := by
         simp [p, q] ; intro k h
@@ -319,19 +319,19 @@ theorem accepted_omega_lang_union :
 
 end  AcceptedLangUnion
 
-section AutomatonProd
+section AutomataProd
 
 variable {I A : Type*}
 
-def AutomatonProd (M : I → Automaton A) : Automaton A where
+def AutomataProd (M : I → Automata A) : Automata A where
   State := Π i : I, (M i).State
   init := { s | ∀ i : I, (s i) ∈ (M i).init }
   next := fun s a ↦ { s' | ∀ i : I, (s' i) ∈ (M i).next (s i) a }
 
-variable (M : I → Automaton A)
+variable (M : I → Automata A)
 
-theorem automaton_prod_fin_run (n : ℕ) (as : Fin n → A) (ss : Fin (n + 1) → (AutomatonProd M).State) :
-    FinRun (AutomatonProd M) n as ss ↔ ∀ i, FinRun (M i) n as (fun k ↦ ss k i) := by
+theorem Automata_prod_fin_run (n : ℕ) (as : Fin n → A) (ss : Fin (n + 1) → (AutomataProd M).State) :
+    FinRun (AutomataProd M) n as ss ↔ ∀ i, FinRun (M i) n as (fun k ↦ ss k i) := by
   constructor
   · rintro ⟨h_init, h_next⟩ i
     constructor
@@ -342,8 +342,8 @@ theorem automaton_prod_fin_run (n : ℕ) (as : Fin n → A) (ss : Fin (n + 1) �
     · intro i ; exact (h_all i).1
     · intro k i ;  exact (h_all i).2 k
 
-theorem automaton_prod_inf_run (as : ℕ → A) (ss : ℕ → (AutomatonProd M).State) :
-    InfRun (AutomatonProd M) as ss ↔ ∀ i, InfRun (M i) as (fun k ↦ ss k i) := by
+theorem Automata_prod_inf_run (as : ℕ → A) (ss : ℕ → (AutomataProd M).State) :
+    InfRun (AutomataProd M) as ss ↔ ∀ i, InfRun (M i) as (fun k ↦ ss k i) := by
   constructor
   · rintro ⟨h_init, h_next⟩ i
     constructor
@@ -354,23 +354,23 @@ theorem automaton_prod_inf_run (as : ℕ → A) (ss : ℕ → (AutomatonProd M).
     · intro i ; exact (h_all i).1
     · intro k i ; exact (h_all i).2 k
 
-end AutomatonProd
+end AutomataProd
 
 section AcceptedLangInter
 
-variable {I A : Type*} (M : I → Automaton A) (acc : (i : I) → Set ((M i).State))
+variable {I A : Type*} (M : I → Automata A) (acc : (i : I) → Set ((M i).State))
 
-def AutomatonProd_Acc : Set (AutomatonProd M).State := { s | ∀ i, (s i) ∈ (acc i) }
+def AutomataProd_Acc : Set (AutomataProd M).State := { s | ∀ i, (s i) ∈ (acc i) }
 
 theorem accepted_lang_inter :
-    AcceptedLang (AutomatonProd M) (AutomatonProd_Acc M acc) = ⋂ i : I, AcceptedLang (M i) (acc i) := by
+    AcceptedLang (AutomataProd M) (AutomataProd_Acc M acc) = ⋂ i : I, AcceptedLang (M i) (acc i) := by
   ext al ; simp [AcceptedLang, FinAccept]
   constructor
   · rintro ⟨n, as, ⟨ss, h_run, h_acc⟩, h_al⟩ i
     use n, as ; simp [h_al]
     use (fun k ↦ ss k i)
     constructor
-    · exact (automaton_prod_fin_run M n as ss).mp h_run i
+    · exact (Automata_prod_fin_run M n as ss).mp h_run i
     · exact h_acc i
   · intro h_all
     have h_all' : ∀ i, ∃ ss_i, FinRun (M i) al.length (fun k ↦ al[k]) ss_i ∧ ss_i (Fin.last al.length) ∈ acc i := by
@@ -391,7 +391,7 @@ theorem accepted_lang_inter :
     choose ss_i h_ss_i using h_all'
     use (fun k i ↦ ss_i i k)
     constructor
-    · apply (automaton_prod_fin_run M al.length (fun k ↦ al[k]) (fun k i ↦ ss_i i k)).mpr
+    · apply (Automata_prod_fin_run M al.length (fun k ↦ al[k]) (fun k i ↦ ss_i i k)).mpr
       intro i
       exact (h_ss_i i).1
     · intro i
@@ -399,68 +399,68 @@ theorem accepted_lang_inter :
 
 end AcceptedLangInter
 
-section AutomatonHist
+section AutomataHist
 
 variable {A H : Type*}
 
-def AutomatonHist (M : Automaton A) (hist_init : Set H) (hist_next : M.State × H → A → Set H) : Automaton A where
+def AutomataHist (M : Automata A) (hist_init : Set H) (hist_next : M.State × H → A → Set H) : Automata A where
   State := M.State × H
   init := { s | s.1 ∈ M.init ∧ s.2 ∈ hist_init }
   next := fun s a ↦ { s' | s'.1 ∈ M.next s.1 a ∧ s'.2 ∈ hist_next s a }
 
-variable (M : Automaton A) (hist_init : Set H) (hist_next : M.State × H → A → Set H)
+variable (M : Automata A) (hist_init : Set H) (hist_next : M.State × H → A → Set H)
 
-theorem automaton_hist_inf_run_proj {as : ℕ → A} {ss : ℕ → M.State × H}
-    (h : InfRun (AutomatonHist M hist_init hist_next) as ss) : InfRun M as (Prod.fst ∘ ss) := by
+theorem Automata_hist_inf_run_proj {as : ℕ → A} {ss : ℕ → M.State × H}
+    (h : InfRun (AutomataHist M hist_init hist_next) as ss) : InfRun M as (Prod.fst ∘ ss) := by
   constructor
   · have h' := h.1
-    simp [AutomatonHist] at h'
+    simp [AutomataHist] at h'
     exact h'.1
   · intro k
     have h' := h.2 k
-    simp [AutomatonHist] at h'
+    simp [AutomataHist] at h'
     exact h'.1
 
 private def _MakeHist (as : ℕ → A) (ss : ℕ → M.State) (hs0 : H) (hs' : M.State × H → A -> H) : ℕ → H
   | 0 => hs0
   | k + 1 => hs' (ss k, _MakeHist as ss hs0 hs' k) (as k)
 
-theorem automaton_hist_inf_run_exists {as : ℕ → A} {ss : ℕ → M.State}
+theorem Automata_hist_inf_run_exists {as : ℕ → A} {ss : ℕ → M.State}
     (h_init : hist_init.Nonempty) (h_next : ∀ s a, (hist_next s a).Nonempty)
-    (h : InfRun M as ss) : ∃ hs : ℕ → H, InfRun (AutomatonHist M hist_init hist_next) as (fun k ↦ (ss k, hs k)) := by
+    (h : InfRun M as ss) : ∃ hs : ℕ → H, InfRun (AutomataHist M hist_init hist_next) as (fun k ↦ (ss k, hs k)) := by
   obtain ⟨hs0, h_hs0⟩ := h_init
   choose hs' h_hs' using h_next
   let hs := _MakeHist M as ss hs0 hs'
   use hs ; constructor
-  · simp [AutomatonHist, _MakeHist, h.1, hs]
+  · simp [AutomataHist, _MakeHist, h.1, hs]
     exact h_hs0
   · intro k
-    simp [AutomatonHist, _MakeHist, hs, h.2 k]
+    simp [AutomataHist, _MakeHist, hs, h.2 k]
     apply h_hs'
 
-end AutomatonHist
+end AutomataHist
 
 section AcceptedOmegaLangInter2
 
 open Classical
 
-variable {A : Type*} (M : Fin 2 → Automaton A) (acc : (i : Fin 2) → Set ((M i).State))
+variable {A : Type*} (M : Fin 2 → Automata A) (acc : (i : Fin 2) → Set ((M i).State))
 
-def AutomatonInter2_HistInit : Set (Fin 2) := {0}
+def AutomataOmegaInter2_HistInit : Set (Fin 2) := {0}
 
-def AutomatonInter2_HistNext : (AutomatonProd M).State × Fin 2 → A → Set (Fin 2) :=
+def AutomataOmegaInter2_HistNext : (AutomataProd M).State × Fin 2 → A → Set (Fin 2) :=
   fun s _ ↦
     if s.1 0 ∈ acc 0 ∧ s.2 = 0 then {1} else
     if s.1 1 ∈ acc 1 ∧ s.2 = 1 then {0} else {s.2}
 
-def AutomatonInter2 : Automaton A :=
-  AutomatonHist (AutomatonProd M) AutomatonInter2_HistInit (AutomatonInter2_HistNext M acc)
+def AutomataOmegaInter2 : Automata A :=
+  AutomataHist (AutomataProd M) AutomataOmegaInter2_HistInit (AutomataOmegaInter2_HistNext M acc)
 
-def AutomatonInter2_Acc : Set (AutomatonInter2 M acc).State :=
+def AutomataOmegaInter2_Acc : Set (AutomataOmegaInter2 M acc).State :=
   { s | s.1 0 ∈ acc 0 ∧ s.2 = 0 } ∪ { s | s.1 1 ∈ acc 1 ∧ s.2 = 1 }
 
-private lemma automaton_inter2_lemma1 {as : ℕ → A} {ss : ℕ → (AutomatonInter2 M acc).State}
-    (h_run : InfRun (AutomatonInter2 M acc) as ss) :
+private lemma Automata_inter2_lemma1 {as : ℕ → A} {ss : ℕ → (AutomataOmegaInter2 M acc).State}
+    (h_run : InfRun (AutomataOmegaInter2 M acc) as ss) :
       (∃ᶠ k in atTop, ss k ∈ { s | s.1 0 ∈ acc 0 ∧ s.2 = 0 }) ↔
       (∃ᶠ k in atTop, ss k ∈ { s | s.1 1 ∈ acc 1 ∧ s.2 = 1 }) := by
   constructor <;> intro h_inf
@@ -470,7 +470,7 @@ private lemma automaton_inter2_lemma1 {as : ℕ → A} {ss : ℕ → (AutomatonI
       apply leads_to_step ; simp [Step]
       intro k h_acc h_hist
       have h_step := (h_run.2 k).2
-      simp [AutomatonInter2_HistNext, h_acc, h_hist] at h_step
+      simp [AutomataOmegaInter2_HistNext, h_acc, h_hist] at h_step
       assumption
     have h_lt2 : LeadsTo ss {s | s.2 = 1} {s | s.1 1 ∈ acc 1 ∧ s.2 = 1} := by
       apply leads_to_until_frequently_1
@@ -479,7 +479,7 @@ private lemma automaton_inter2_lemma1 {as : ℕ → A} {ss : ℕ → (AutomatonI
         rw [imp_not_comm] at h_acc
         have h_acc := h_acc h_hist
         have h_step := (h_run.2 k).2
-        simp [AutomatonInter2_HistNext, h_acc, h_hist] at h_step
+        simp [AutomataOmegaInter2_HistNext, h_acc, h_hist] at h_step
         assumption
       · let p k := ss k ∈ {s | s.1 0 ∈ acc 0 ∧ s.2 = 0}
         let q k := ss k ∉ {s | s.2 = 1}
@@ -494,7 +494,7 @@ private lemma automaton_inter2_lemma1 {as : ℕ → A} {ss : ℕ → (AutomatonI
       apply leads_to_step ; simp [Step]
       intro k h_acc h_hist
       have h_step := (h_run.2 k).2
-      simp [AutomatonInter2_HistNext, h_acc, h_hist] at h_step
+      simp [AutomataOmegaInter2_HistNext, h_acc, h_hist] at h_step
       assumption
     have h_lt2 : LeadsTo ss {s | s.2 = 0} {s | s.1 0 ∈ acc 0 ∧ s.2 = 0} := by
       apply leads_to_until_frequently_1
@@ -503,7 +503,7 @@ private lemma automaton_inter2_lemma1 {as : ℕ → A} {ss : ℕ → (AutomatonI
         rw [imp_not_comm] at h_acc
         have h_acc := h_acc h_hist
         have h_step := (h_run.2 k).2
-        simp [AutomatonInter2_HistNext, h_acc, h_hist] at h_step
+        simp [AutomataOmegaInter2_HistNext, h_acc, h_hist] at h_step
         assumption
       · let p k := ss k ∈ {s | s.1 1 ∈ acc 1 ∧ s.2 = 1}
         let q k := ss k ∉ {s | s.2 = 0}
@@ -513,26 +513,26 @@ private lemma automaton_inter2_lemma1 {as : ℕ → A} {ss : ℕ → (AutomatonI
         exact Frequently.mono h_inf h_imp
     exact leads_to_trans h_lt1 h_lt2
 
-private lemma automaton_inter2_lemma2 {as : ℕ → A} {ss : ℕ → (AutomatonInter2 M acc).State}
-    (h_run : InfRun (AutomatonInter2 M acc) as ss)
+private lemma Automata_inter2_lemma2 {as : ℕ → A} {ss : ℕ → (AutomataOmegaInter2 M acc).State}
+    (h_run : InfRun (AutomataOmegaInter2 M acc) as ss)
     (h_inf0 : ∃ᶠ k in atTop, ss k ∈ { s | s.1 0 ∈ acc 0 })
     (h_inf1 : ∃ᶠ k in atTop, ss k ∈ { s | s.1 1 ∈ acc 1 }) :
       ∃ᶠ k in atTop, ss k ∈ { s | s.1 0 ∈ acc 0 ∧ s.2 = 0 } ∪ { s | s.1 1 ∈ acc 1 ∧ s.2 = 1 } := by
   have h_true : ∃ᶠ k in atTop, ss k ∈ univ := by simp [atTop_neBot]
   apply frequently_leads_to_frequently h_true
   apply leads_to_cases (p := univ) (q := {s | s.2 = 0}) <;> simp [univ_inter]
-  · have h_inter : {s : (AutomatonInter2 M acc).State | s.1 0 ∈ acc 0 ∧ s.2 = 0} = {s | s.2 = 0} ∩ {s | s.1 0 ∈ acc 0} := by
+  · have h_inter : {s : (AutomataOmegaInter2 M acc).State | s.1 0 ∈ acc 0 ∧ s.2 = 0} = {s | s.2 = 0} ∩ {s | s.1 0 ∈ acc 0} := by
       ext s ; simp ; tauto
     rw [h_inter]
     apply leads_to_until_frequently_2 (h2 := h_inf0)
     simp [Step]
     intro k h_hist h_acc
     have h_step := (h_run.2 k).2
-    simp [AutomatonInter2_HistNext, h_acc, h_hist] at h_step
+    simp [AutomataOmegaInter2_HistNext, h_acc, h_hist] at h_step
     assumption
-  · have h_inter : {s : (AutomatonInter2 M acc).State | s.1 1 ∈ acc 1 ∧ s.2 = 1} = {s | s.2 = 1} ∩ {s | s.1 1 ∈ acc 1} := by
+  · have h_inter : {s : (AutomataOmegaInter2 M acc).State | s.1 1 ∈ acc 1 ∧ s.2 = 1} = {s | s.2 = 1} ∩ {s | s.1 1 ∈ acc 1} := by
       ext s ; simp ; tauto
-    have h_compl : {s : (AutomatonInter2 M acc).State | s.2 = 0}ᶜ = {s | s.2 = 1} := by
+    have h_compl : {s : (AutomataOmegaInter2 M acc).State | s.2 = 0}ᶜ = {s | s.2 = 1} := by
       ext s ; simp
       constructor
       · exact Fin.eq_one_of_neq_zero s.2
@@ -542,16 +542,16 @@ private lemma automaton_inter2_lemma2 {as : ℕ → A} {ss : ℕ → (AutomatonI
     simp [Step]
     intro k h_hist h_acc
     have h_step := (h_run.2 k).2
-    simp [AutomatonInter2_HistNext, h_acc, h_hist] at h_step
+    simp [AutomataOmegaInter2_HistNext, h_acc, h_hist] at h_step
     assumption
 
 theorem accepted_omega_lang_inter2 :
-    AcceptedOmegaLang (AutomatonInter2 M acc) (AutomatonInter2_Acc M acc) = ⋂ i : Fin 2, AcceptedOmegaLang (M i) (acc i) := by
+    AcceptedOmegaLang (AutomataOmegaInter2 M acc) (AutomataOmegaInter2_Acc M acc) = ⋂ i : Fin 2, AcceptedOmegaLang (M i) (acc i) := by
   ext as ; simp [AcceptedOmegaLang, BuchiAccept]
   constructor
   · rintro ⟨ss, h_run, h_inf⟩ i
-    have h_run1 := automaton_hist_inf_run_proj (AutomatonProd M) AutomatonInter2_HistInit (AutomatonInter2_HistNext M acc) h_run
-    have h_run' := (automaton_prod_inf_run M as (Prod.fst ∘ ss)).mp h_run1 i
+    have h_run1 := Automata_hist_inf_run_proj (AutomataProd M) AutomataOmegaInter2_HistInit (AutomataOmegaInter2_HistNext M acc) h_run
+    have h_run' := (Automata_prod_inf_run M as (Prod.fst ∘ ss)).mp h_run1 i
     use (fun k ↦ (Prod.fst ∘ ss) k i) ; constructor
     · assumption
     let p0 k := ss k ∈ { s | s.1 0 ∈ acc 0 ∧ s.2 = 0 }
@@ -566,23 +566,23 @@ theorem accepted_omega_lang_inter2 :
     constructor <;> intro h_run_i
     · rcases h_inf_or with h_inf0 | h_inf1
       · exact Frequently.mono h_inf0 h_p0_p0'
-      · rw [← automaton_inter2_lemma1 M acc h_run] at h_inf1
+      · rw [← Automata_inter2_lemma1 M acc h_run] at h_inf1
         exact Frequently.mono h_inf1 h_p0_p0'
     · rcases h_inf_or with h_inf0 | h_inf1
-      · rw [automaton_inter2_lemma1 M acc h_run] at h_inf0
+      · rw [Automata_inter2_lemma1 M acc h_run] at h_inf0
         exact Frequently.mono h_inf0 h_p1_p1'
       · exact Frequently.mono h_inf1 h_p1_p1'
   · intro h_all
     choose ss h_ss using h_all
     let ss' := fun k i ↦ ss i k
     have h_ss' : ∀ i, InfRun (M i) as (fun k ↦ ss' k i) := by intro i ; exact (h_ss i).1
-    have h_run' := (automaton_prod_inf_run M as ss').mpr h_ss'
-    have h_hist_init : AutomatonInter2_HistInit.Nonempty := by simp [AutomatonInter2_HistInit]
-    have h_hist_next : ∀ s a, (AutomatonInter2_HistNext M acc s a).Nonempty := by
-      intro s a ; simp only [AutomatonInter2_HistNext]
+    have h_run' := (Automata_prod_inf_run M as ss').mpr h_ss'
+    have h_hist_init : AutomataOmegaInter2_HistInit.Nonempty := by simp [AutomataOmegaInter2_HistInit]
+    have h_hist_next : ∀ s a, (AutomataOmegaInter2_HistNext M acc s a).Nonempty := by
+      intro s a ; simp only [AutomataOmegaInter2_HistNext]
       rcases Classical.em (s.1 0 ∈ acc 0 ∧ s.2 = 0) with cond1 | cond1 <;> simp [cond1]
       rcases Classical.em (s.1 1 ∈ acc 1 ∧ s.2 = 1) with cond2 | cond2 <;> simp [cond2]
-    have h_runh := automaton_hist_inf_run_exists (AutomatonProd M) AutomatonInter2_HistInit (AutomatonInter2_HistNext M acc)
+    have h_runh := Automata_hist_inf_run_exists (AutomataProd M) AutomataOmegaInter2_HistInit (AutomataOmegaInter2_HistNext M acc)
       h_hist_init h_hist_next h_run'
     obtain ⟨hs, h_run⟩ := h_runh
     use (fun k ↦ (ss' k, hs k))
@@ -590,6 +590,6 @@ theorem accepted_omega_lang_inter2 :
     · assumption
     have h_inf0 : ∃ᶠ k in atTop, ss' k ∈ { s | s 0 ∈ acc 0 } := by simp [ss', (h_ss 0).2]
     have h_inf1 : ∃ᶠ k in atTop, ss' k ∈ { s | s 1 ∈ acc 1 } := by simp [ss', (h_ss 1).2]
-    exact automaton_inter2_lemma2 M acc h_run h_inf0 h_inf1
+    exact Automata_inter2_lemma2 M acc h_run h_inf0 h_inf1
 
 end AcceptedOmegaLangInter2
